started kernel verification

InvIfScript.sml
@@ -3,7 +3,9 @@
 open HolKernel boolLib bossLib;
 open wordsLib blastLib; 
 
+open basetypesTheory;
 open hwTheory;
+open cachelessTheory;
 
 val _ = new_theory "InvIf";
 
@@ -87,9 +89,7 @@ val Icoh_dCoh_po = Define `Icoh_dCoh_po I =
 `;
 
 val Icode_CR_po = Define `Icode_CR_po I = 
-!s s'. dCoh s.ms {pa | MEM pa IN CR s} 
-    /\ dCoh s'.ms {pa | MEM pa IN CR s'}
-    /\ iCoh s.ms {pa | MEM pa IN CRex s}
+!s s'. iCoh s.ms {pa | MEM pa IN CRex s}
     /\ iCoh s'.ms {pa | MEM pa IN CRex s'}
     /\ isafe s {pa | MEM pa IN CRex s}
     /\ isafe s' {pa | MEM pa IN CRex s'}
@@ -147,7 +147,7 @@ val Icoh_exists = store_thm("Icoh_exists", ``
   RW_TAC std_ss [Icoh_dCoh_po, Icoh_CR_po]
 );
 
-val Icode_exists = store_thm("Icoh_exists", ``
+val Icode_exists = store_thm("Icode_exists", ``
 ?Icode. Icode_CR_po Icode /\ Icode_iCoh_po Icode /\ Icode_isafe_po Icode
 ``,
   EXISTS_TAC ``\s. iCoh s.ms {pa | MEM pa IN CRex s}
@@ -232,9 +232,7 @@ val Icoh_dCoh_oblg = store_thm("Icoh_dCoh_oblg", ``
 ); 
 
 val Icode_CR_oblg = store_thm("Icode_CR_oblg", ``
-!s s'. dCoh s.ms {pa | MEM pa IN CR s} 
-    /\ dCoh s'.ms {pa | MEM pa IN CR s'}
-    /\ iCoh s.ms {pa | MEM pa IN CRex s}
+!s s'. iCoh s.ms {pa | MEM pa IN CRex s}
     /\ iCoh s'.ms {pa | MEM pa IN CRex s'}
     /\ isafe s {pa | MEM pa IN CRex s}
     /\ isafe s' {pa | MEM pa IN CRex s'}
@@ -282,6 +280,273 @@ val Inv_oblg = store_thm("Inv_oblg", ``
   ASSUME_TAC Inv_spec >>
   FULL_SIMP_TAC std_ss []
 ); 
+
+(******** Simulation relation ********)
+
+val Mv_def = Define `
+   (Mv sc (MEM pa) = dmvalt sc.ms T pa)
+/\ (Mv sc r = Cv sc r)
+`;
+
+val Rsim_def = Define `Rsim sc s = 
+!r. cl_Cv s r = Mv sc r
+`;
+
+val Rsim_lem = store_thm("Rsim_lem", ``
+!sc s. Rsim sc s <=>    (!r. reg_res r ==> (cl_Cv s r = Cv sc r)) 
+                     /\ (!pa. MVcl s.M T pa = dmvalt sc.ms T pa)
+``,
+  RW_TAC std_ss [Rsim_def] >>
+  EQ_TAC 
+  >| [(* ==> *)
+      REPEAT STRIP_TAC
+      >| [(* register *)
+	  PAT_X_ASSUM ``!r. x`` (
+	      fn thm => ASSUME_TAC ( SPEC ``r:resource`` thm )
+	  ) >>
+	  Cases_on `r` >> ( 
+	      FULL_SIMP_TAC std_ss [Mv_def, coreIfTheory.reg_res_def] 
+	  ) 
+	  ,
+	  (* memory *)
+	  PAT_X_ASSUM ``!r. x`` (
+	      fn thm => ASSUME_TAC ( SPEC ``MEM pa`` thm )
+	  ) >>
+	  FULL_SIMP_TAC std_ss [cl_Cv_def, Mv_def, coreIfTheory.CV_def]
+	 ]
+      ,
+      (* <== *)
+      REPEAT STRIP_TAC >>
+      Cases_on `r` >> (
+          FULL_SIMP_TAC std_ss [cl_Cv_def, Mv_def, 
+				coreIfTheory.reg_res_def,
+				coreIfTheory.CV_def]
+      )
+     ]	  
+);
+
+val Rsim_dCoh_lem = store_thm("Rsim_dCoh_lem", ``
+!sc s As. Rsim sc s /\ dCoh sc.ms As ==>
+    !pa. pa IN As ==> (MVcl s.M T pa = dmvca sc.ms T pa)
+``,
+  RW_TAC std_ss [Rsim_lem, dCoh_alt_lem]
+);
+
+val Rsim_iCoh_lem = store_thm("Rsim_iCoh_lem", ``
+!sc s As. Rsim sc s /\ dCoh sc.ms As /\ iCoh sc.ms As ==>
+    !pa. pa IN As /\ ~dirty sc.ms pa ==> (MVcl s.M T pa = imv sc.ms T pa)
+``,
+  RW_TAC std_ss [Rsim_lem] >>
+  IMP_RES_TAC dCoh_alt_lem >>
+  IMP_RES_TAC dCoh_lem >>
+  IMP_RES_TAC msIfTheory.iCoh_def >>
+  IMP_RES_TAC imv_dmv_lem >>
+  RW_TAC std_ss []
+);
+
+
+(******** Cache-less Invariants and proof obligations **********)
+
+(* critical resources *)
+
+val cl_CR_def = Define `cl_CR s = CR_(s.cs, MVcl s.M)`;
+
+val cl_CR_lem = store_thm("cl_CR_lem", ``
+!s sca. (!r. r IN cl_CR s ==> (cl_Cv s r = Cv sca r)) ==>
+    (cl_CR s = CR sca)
+``,
+  RW_TAC std_ss [cl_CR_def, CR_def, cl_Cv_def, Cv_def] >>
+  IMP_RES_TAC CR_spec
+);
+
+val CR_cl_lem = store_thm("CR_cl_lem", ``
+!s sca. (!r. r IN CR sca ==> (cl_Cv s r = Cv sca r)) ==>
+    (cl_CR s = CR sca)
+``,
+  RW_TAC std_ss [cl_CR_def, CR_def, cl_Cv_def, Cv_def] >>
+  METIS_TAC [CR_spec]
+);
+
+val cl_MD_lem = store_thm("cl_CR_lem", ``
+!s sca. (!r. r IN cl_MD s ==> (cl_Cv s r = Cv sca r)) ==>
+    (cl_MD s = MD sca)
+``,
+  RW_TAC std_ss [cl_MD_def, MD_def, cl_Cv_def, Cv_def] >>
+  IMP_RES_TAC MD__lem
+);
+
+val MD_cl_lem = store_thm("CR_cl_lem", ``
+!s sca. (!r. r IN MD sca ==> (cl_Cv s r = Cv sca r)) ==>
+    (cl_MD s = MD sca)
+``,
+  RW_TAC std_ss [cl_MD_def, MD_def, cl_Cv_def, Cv_def] >>
+  METIS_TAC [MD__lem]
+);
+
+(* software invariants *)
+
+val cl_Inv_exists = store_thm("cl_Inv_exists", ``
+?cl_Inv.
+!s sca. (!r. r IN cl_CR s ==> (cl_Cv s r = Cv sca r)) ==>
+    (cl_Inv s <=> Ifun sca)
+``,
+  EXISTS_TAC ``\s.
+      !sca. (!r. r IN cl_CR s ==> (cl_Cv s r = Cv sca r)) ==> Ifun sca`` >>
+  RW_TAC std_ss [] >>
+  EQ_TAC
+  >| [(* ==> *)
+      REPEAT STRIP_TAC >>
+      PAT_X_ASSUM ``!sca'. x ==> Ifun sca'`` (
+          fn thm => ASSUME_TAC ( SPEC ``sca:hw_state`` thm )
+      ) >>
+      FULL_SIMP_TAC std_ss []
+      ,
+      (* <== *)
+      REPEAT STRIP_TAC >>
+      IMP_RES_TAC cl_CR_lem >>
+      FULL_SIMP_TAC std_ss [] >>
+      IMP_RES_TAC Ifun_CR_oblg
+     ]
+);
+
+val cl_Inv_spec = new_specification ("cl_Inv_spec",
+  ["cl_Inv"], cl_Inv_exists);
+
+val cl_Inv_preserve_po = Define `cl_Inv_preserve_po =
+!s s'. cl_Inv s /\ cl_wrel s s' ==> cl_Inv s'
+`;
+
+(* NOTE: omitting Kvm and PC condition here, 
+ * just need:
+ ** executable addresses are in CR
+ ** only cacheable addresses are used 
+ ** PRIV configuration not changed by kernel (needed to couple Mon)
+TODO?: pc always at executable address -> 
+   avoids nexted exceptions, not modeled here, not important for proof
+*)
+val cl_Inv_Mmu_po = Define `cl_Inv_Mmu_po = 
+!s s' n. cl_Inv s /\ cl_kcomp s s' n ==>
+    (!va pa c acc. (Mmu_(s.cs, MVcl s.M, va, PRIV, acc) = SOME (pa,c)) ==>
+                   ((acc = EX) ==> MEM pa IN cl_CR s) /\ (c = T))
+ /\ (!va acc. Mmu_(s'.cs, MVcl s'.M, va, PRIV, acc) = 
+              Mmu_(s.cs, MVcl s.M, va, PRIV, acc))
+`;
+
+(* some lemmas *)
+
+val cl_Inv_Mmu_lem = store_thm("cl_Inv_Mmu_req_lem", ``
+!s s' req s'' n. cl_Inv_Mmu_po /\ cl_Inv s /\ cl_kcomp s s' n 
+        ==>
+    (!va pa c acc. (Mmu_(s'.cs, MVcl s'.M, va, PRIV, acc) = SOME (pa,c)) ==>
+                   ((acc = EX) ==> MEM pa IN cl_CR s) /\ (c = T))
+``,
+  REPEAT GEN_TAC >>
+  STRIP_TAC >>
+  REPEAT GEN_TAC >>
+  IMP_RES_TAC cl_Inv_Mmu_po >>
+  ASM_REWRITE_TAC [] >>
+  STRIP_TAC >>
+  RES_TAC >>
+  ASM_REWRITE_TAC []
+);
+
+val cl_Inv_Mmu_req_lem = store_thm("cl_Inv_Mmu_req_lem", ``
+!s s' req s'' n. cl_Inv_Mmu_po /\ cl_Inv s /\ req <> NOREQ 
+	      /\ cl_kcomp s s' n /\ cl_trans s' PRIV req s''
+        ==>
+    (Freq req ==> MEM (Adr req) IN cl_CR s) /\ CAreq req
+``,
+  REPEAT GEN_TAC >>
+  STRIP_TAC >>
+  IMP_RES_TAC cl_trans_core_req_lem >>
+  IMP_RES_TAC core_req_mmu_lem >>
+  IMP_RES_TAC cl_Inv_Mmu_lem >>
+  ASM_REWRITE_TAC [] >>
+  IMP_RES_TAC not_NOREQ_lem
+  >| [(* Dreq *)
+      IMP_RES_TAC Dreq_lem >>
+      RW_TAC std_ss [Freq_def]
+      ,
+      (* Freq *)
+      IMP_RES_TAC Freq_lem >>
+      FULL_SIMP_TAC std_ss [Acc_def]
+     ]
+);
+
+val Rsim_CR_lem = store_thm("Rsim_CR_lem", ``
+!sc s. Rsim sc s /\ Icoh sc ==>
+    (!r. r IN CR sc ==> (cl_Cv s r = Cv sc r))
+``,
+  REPEAT STRIP_TAC >>
+  Cases_on `reg_res r`
+  >| [(* register *)
+      FULL_SIMP_TAC std_ss [Rsim_lem]
+      ,
+      (* memory *)
+      ASSUME_TAC ( SPEC ``r:resource`` coreIfTheory.res_cases ) >>
+      FULL_SIMP_TAC std_ss [] >> (
+          FULL_SIMP_TAC std_ss [] 
+      ) >>
+      IMP_RES_TAC Icoh_dCoh_oblg >>
+      `pa IN {pa | MEM pa IN CR sc}` by (
+          FULL_SIMP_TAC std_ss [pred_setTheory.IN_GSPEC_IFF]
+      ) >>
+      IMP_RES_TAC Rsim_dCoh_lem >>
+      RW_TAC std_ss [cl_Cv_def, Cv_def, coreIfTheory.CV_def]
+     ]
+);
+
+val Rsim_cl_CR_lem = store_thm("Rsim_CR_lem", ``
+!sc s. Rsim sc s /\ Icoh sc ==>
+    (!r. r IN cl_CR s ==> (cl_Cv s r = Cv sc r))
+``,
+  REPEAT STRIP_TAC >>
+  IMP_RES_TAC Rsim_CR_lem >>
+  IMP_RES_TAC CR_cl_lem >>
+  FULL_SIMP_TAC std_ss []
+);
+
+val Rsim_MD_lem = store_thm("Rsim_MD_lem", ``
+!sc s. Rsim sc s /\ Icoh sc /\ Ifun sc ==>
+    (!r. cl_MD s = MD sc)
+``,
+  REPEAT STRIP_TAC >>
+  IMP_RES_TAC Rsim_CR_lem >>
+  MATCH_MP_TAC MD_cl_lem >>
+  REPEAT STRIP_TAC >>
+  IMP_RES_TAC Ifun_MD_oblg >>
+  RES_TAC 
+);
+
+
+val Rsim_Mon_lem = store_thm("Rsim_Mon_lem", ``
+!sc s. Rsim sc s /\ Icoh sc /\ Ifun sc ==>
+    (!r m ac. cl_Mon s r m ac = Mon sc r m ac)
+``,
+  RW_TAC std_ss [cl_Mon_def, Mon_def] >>
+  MATCH_MP_TAC Mon__lem >>
+  REPEAT STRIP_TAC >>
+  IMP_RES_TAC Rsim_MD_lem >>
+  IMP_RES_TAC Ifun_MD_oblg >>
+  FULL_SIMP_TAC std_ss [cl_MD_def, MD_def] >>
+  RES_TAC >>
+  IMP_RES_TAC Rsim_CR_lem >>
+  FULL_SIMP_TAC std_ss [cl_Cv_def, Cv_def]
+);
+
+(* internal invariants *)
+
+val cmfinv_xfer_def = Define `cmfinv_xfer Ic I =
+!sc sc' s s'. Inv sc /\ cl_Inv s /\ Icoh sc' /\ Icode sc' 
+           /\ Rsim sc s /\ Rsim sc' s'
+        ==>
+    (Ic sc sc' <=> I s s')
+`;
+
+val cmfinv_sinv_def = Define `cmfinv_sinv If Is =
+!sc sc'. Inv sc /\ Icoh sc' /\ Icode sc' /\ If sc sc' ==> Is sc'
+`;
+
 
 
 (*********** finish ************)
