cachelessScript.sml
@@ -1,0 +1,334 @@
+(********** Loading *************)
+
+open HolKernel boolLib bossLib;
+open wordsLib blastLib; 
+
+open basetypesTheory;
+open hwTheory;
+
+val _ = new_theory "cacheless";
+
+(********* cacheless state **********)
+
+val _ = Datatype `cl_state = <| 
+    cs  : core_state;
+    M  : mem_state
+|>`;
+
+val cl_MD_def = Define `cl_MD s = MD_ (s.cs, MVcl s.M)`;
+val cl_Mon_def = Define `cl_Mon s r m ac = Mon_ (s.cs, MVcl s.M, r, m, ac)`;
+val cl_Mmu_def = Define `cl_Mmu s va m ac = Mmu_ (s.cs, MVcl s.M, va, m, ac)`;
+val cl_Cv_def = Define `cl_Cv s r = CV s.cs (MVcl s.M) r`;
+val cl_mode_def = Define `cl_mode s = Mode s.cs`;
+val cl_exentry_def = Define `cl_exentry s = exentry_ s.cs`;
+
+val cl_Mon_lem = store_thm("cl_Mon_lem", ``
+!s s'. (!r. r IN cl_MD s ==> (cl_Cv s r = cl_Cv s' r)) ==>
+       (!r m ac. cl_Mon s r m ac <=> cl_Mon s' r m ac)
+``,
+  RW_TAC std_ss [cl_MD_def, cl_Mon_def, cl_Cv_def] >>
+  RW_TAC std_ss [Mon__lem]
+);
+
+val cl_MD_lem = store_thm("cl_MD_lem", ``
+!s s'. (!r. r IN cl_MD s ==> (cl_Cv s r = cl_Cv s' r)) ==> (cl_MD s = cl_MD s')
+``,
+  RW_TAC std_ss [cl_MD_def, cl_Cv_def, MD__lem]
+);
+
+val (cl_trans_rules, cl_trans_ind, cl_trans_cases) = Hol_reln `
+   (!s M dop cs' s'. 
+	rd dop 
+     /\ (M = Mode s.cs)
+     /\ core_req (s.cs, M, MVcl s.M, DREQ dop, cs') 
+     /\ (s'.M = mtfcl s.M dop)
+     /\ core_rcv (cs', M, MVcl s.M (CA dop) (PA dop), s'.cs)
+    ==>
+    cl_trans s M (DREQ dop) s')
+/\ (!s M dop s'. 
+	~rd dop 
+     /\ (M = Mode s.cs)
+     /\ core_req (s.cs, M, MVcl s.M, DREQ dop, s'.cs) 
+     /\ (s'.M = mtfcl s.M dop)
+    ==>
+    cl_trans s M (DREQ dop) s')
+/\ (!s M pa cs' s'. 
+        (M = Mode s.cs)
+     /\ core_req (s.cs, M, MVcl s.M, FREQ pa, cs') 
+     /\ (s'.M = mtfcl s.M (RD pa T))
+     /\ core_rcv (cs', M, MVcl s.M T pa, s'.cs)
+    ==>
+    cl_trans s M (FREQ pa) s')
+/\ (!s M s'. 
+        (M = Mode s.cs)
+     /\ core_req (s.cs, M, MVcl s.M, NOREQ, s'.cs)
+     /\ (s'.M = s.M)
+    ==>
+    cl_trans s M NOREQ s')
+`;
+
+(* cl_trans lemmas *)
+
+val cl_trans_mode_not_eq_lem = store_thm("cl_trans_mode_not_eq_lem", ``
+!s M req s'. (M <> Mode s.cs) ==> ~cl_trans s M req s' 
+``,
+  REPEAT STRIP_TAC >>
+  IMP_RES_TAC cl_trans_cases
+); 
+
+val cl_trans_mode_lem = 
+cl_trans_mode_not_eq_lem |> SPEC_ALL 
+			 |> CONTRAPOS 
+			 |> GEN_ALL 
+			 |> SIMP_RULE std_ss [];
+
+val cl_trans_fetch_lem = store_thm("cl_trans_fetch_lem", ``
+!s M req s'. Freq req /\ cl_trans s M req s' ==>
+?cs'. core_req (s.cs, M, MVcl s.M, req, cs') 
+   /\ (s'.M = mtfcl s.M (Dop req))
+   /\ core_rcv (cs', M, MVcl s.M T (Adr req), s'.cs)
+``,
+  REPEAT STRIP_TAC >>
+  IMP_RES_TAC Freq_lem >>
+  RW_TAC std_ss [Adr_def, Dop_def] >>
+  IMP_RES_TAC cl_trans_cases >> (
+      FULL_SIMP_TAC std_ss [corereq_distinct]
+  ) >>
+  FULL_SIMP_TAC std_ss [corereq_11] >>
+  RW_TAC std_ss [] >>
+  HINT_EXISTS_TAC >>
+  RW_TAC std_ss []
+);
+
+val cl_trans_data_lem = store_thm("cl_trans_data_lem", ``
+!s M req s'. Dreq req /\ cl_trans s M req s' ==> 
+    (s'.M = mtfcl s.M (Dop req))
+``,
+  REPEAT STRIP_TAC >>
+  IMP_RES_TAC Dreq_lem >>
+  RW_TAC std_ss [Dop_def] >>
+  IMP_RES_TAC cl_trans_cases >> (
+      FULL_SIMP_TAC std_ss [corereq_distinct, corereq_11]
+  )
+);
+
+val cl_trans_core_req_lem = store_thm("cl_trans_core_req_lem", ``
+!s M req s'. cl_trans s M req s' ==> 
+    ?cs'. core_req (s.cs, M, MVcl s.M, req, cs') 
+``,
+  REPEAT STRIP_TAC >>
+  IMP_RES_TAC cl_trans_cases >> (
+      FULL_SIMP_TAC std_ss [corereq_distinct] >>
+      REV_FULL_SIMP_TAC std_ss [] >>
+      HINT_EXISTS_TAC >>
+      RW_TAC std_ss []
+  )
+);
+
+val cl_trans_read_lem = store_thm("cl_trans_read_lem", ``
+!s M req s'. Rreq req /\ cl_trans s M req s' ==>
+?cs'. core_req (s.cs, M, MVcl s.M, req, cs') 
+   /\ (s'.M = s.M)
+   /\ core_rcv (cs', M, MVcl s.M (CAreq req) (Adr req), s'.cs)
+``,
+  REPEAT STRIP_TAC >>
+  IMP_RES_TAC Rreq_lem >>
+  RW_TAC std_ss [CAreq_def, Adr_def, Dop_def] >>
+  IMP_RES_TAC cl_trans_cases >> (
+      FULL_SIMP_TAC std_ss [corereq_distinct, corereq_11] >>
+      REV_FULL_SIMP_TAC std_ss []
+  ) >>
+  HINT_EXISTS_TAC >>
+  IMP_RES_TAC rd_lem >>
+  RW_TAC std_ss [cachememTheory.mtfcl_def]
+);
+
+val cl_trans_write_lem = store_thm("cl_trans_write_lem", ``
+!s M req s'. Wreq req /\ cl_trans s M req s' ==>
+    core_req (s.cs, M, MVcl s.M, req, s'.cs) 
+ /\ (s'.M = mtfcl s.M (Dop req))
+``,
+  REPEAT GEN_TAC >>
+  STRIP_TAC >>
+  IMP_RES_TAC Wreq_lem >>
+  ASM_REWRITE_TAC [Dop_def] >>
+  IMP_RES_TAC not_rd_lem >>
+  RW_TAC std_ss [] >> (
+      IMP_RES_TAC cl_trans_cases >> (
+          FULL_SIMP_TAC std_ss [corereq_distinct, corereq_11] >>
+	  REV_FULL_SIMP_TAC std_ss []
+      )
+  )
+);
+
+val cl_trans_clean_lem = store_thm("cl_trans_clean_lem", ``
+!s M req s'. Creq req /\ cl_trans s M req s' ==>
+    core_req (s.cs, M, MVcl s.M, req, s'.cs) 
+ /\ (s'.M = s.M)
+``,
+  REPEAT GEN_TAC >>
+  STRIP_TAC >>
+  IMP_RES_TAC Creq_lem >>
+  ASM_REWRITE_TAC [] >>
+  IMP_RES_TAC not_rd_lem >>
+  RW_TAC std_ss [] >> (
+      IMP_RES_TAC cl_trans_cases >> (
+          FULL_SIMP_TAC std_ss [corereq_distinct, corereq_11] >>
+          REV_FULL_SIMP_TAC std_ss []
+      )
+  ) >>
+  IMP_RES_TAC cl_lem >>
+  FULL_SIMP_TAC std_ss [cachememTheory.mtfcl_def]
+);
+
+val cl_trans_noreq_lem = store_thm("cl_trans_noreq_lem", ``
+!s M s'. cl_trans s M NOREQ s' ==>
+    core_req (s.cs, M, MVcl s.M, NOREQ, s'.cs) /\ (s'.M = s.M)
+``,
+  REPEAT GEN_TAC >>
+  STRIP_TAC >>
+  IMP_RES_TAC cl_trans_cases >> (
+      FULL_SIMP_TAC std_ss [corereq_distinct]
+  )
+);
+
+val cl_trans_not_Dreq_lem = store_thm("cl_trans_not_Dreq_lem", ``
+!s m req s'. ~Dreq req /\ cl_trans s m req s' ==>
+    !pa. s'.M pa = s.M pa
+``,
+  REPEAT GEN_TAC >>
+  STRIP_TAC >>
+  `Freq req \/ (req = NOREQ)` by ( METIS_TAC [req_cases_lem] ) 
+  >| [(* fetch *)
+      IMP_RES_TAC cl_trans_fetch_lem >>
+      IMP_RES_TAC Freq_lem >>
+      FULL_SIMP_TAC std_ss [Dop_def] >>
+      RW_TAC std_ss [cachememTheory.mtfcl_def]
+      ,
+      (* NOREQ *)
+      FULL_SIMP_TAC std_ss [] >>
+      IMP_RES_TAC cl_trans_noreq_lem >>
+      FULL_SIMP_TAC std_ss [] 
+     ]
+);
+
+val cl_trans_not_write_lem = store_thm("cl_trans_not_write_lem", ``
+!s m req s' pa. (Wreq req ==> Adr req <> pa) /\ cl_trans s m req s' ==>
+    (cl_Cv s' (MEM pa) = cl_Cv s (MEM pa))
+``,
+  RW_TAC std_ss [cl_Cv_def, coreIfTheory.CV_def, cachememTheory.MVcl_def] >>
+  Cases_on `Dreq req` 
+  >| [(* Dreq *)
+      IMP_RES_TAC Dreq_cases_lem 
+      >| [(* read *)
+	  IMP_RES_TAC cl_trans_read_lem >>
+	  ASM_REWRITE_TAC []
+	  ,
+	  (* write *)
+	  IMP_RES_TAC cl_trans_write_lem >>
+	  RES_TAC >>
+	  IMP_RES_TAC Wreq_lem >>
+	  FULL_SIMP_TAC std_ss [Adr_def, Dop_def] >>
+	  IMP_RES_TAC cachememTheory.cl_other_unchanged_lem >>
+	  METIS_TAC []
+	  ,
+	  (* clean *)
+	  IMP_RES_TAC cl_trans_clean_lem >>
+	  ASM_REWRITE_TAC []
+	 ]
+      ,
+      (* not Dreq *)
+      IMP_RES_TAC cl_trans_not_Dreq_lem >>
+      FULL_SIMP_TAC std_ss [] 
+     ]
+);
+
+val cl_trans_not_write_lem2 = store_thm("cl_trans_not_write_lem2", ``
+!s m req s' pa. ~(Wreq req /\ (Adr req = pa)) /\ cl_trans s m req s' ==>
+    (cl_Cv s' (MEM pa) = cl_Cv s (MEM pa))
+``,
+  METIS_TAC [cl_trans_not_write_lem]
+);
+
+val cl_trans_mon_lem = store_thm("cl_trans_mon_lem", ``
+!s M req s'. req <> NOREQ /\ cl_trans s M req s' ==>
+    cl_Mon s (MEM (Adr req)) M (Acc req)
+``,
+  RW_TAC std_ss [cl_Mon_def] >>
+  IMP_RES_TAC not_NOREQ_lem 
+  >| [(* Dreq *)
+      IMP_RES_TAC Dreq_cases_lem
+      >| [(* read *)
+	  IMP_RES_TAC cl_trans_read_lem
+	  ,
+	  (* write *)
+	  IMP_RES_TAC cl_trans_write_lem
+	  ,
+	  (* clean *)
+	  IMP_RES_TAC cl_trans_clean_lem 
+	 ] >> (
+          IMP_RES_TAC core_req_mem_req_lem
+      )
+      ,
+      (* Freq *)
+      IMP_RES_TAC cl_trans_fetch_lem >> 
+      IMP_RES_TAC core_req_mem_req_lem
+     ]
+);
+
+(********* cacheless computation **********)
+
+val (cl_kcomp_rules, cl_kcomp_ind, cl_kcomp_cases) = Hol_reln `
+   (!s. cl_exentry s ==> cl_kcomp s s 0)
+/\ (!s s' s'' n. cl_kcomp s s' n /\ (?req. cl_trans s' PRIV req s'')
+        ==>
+    cl_kcomp s s'' (SUC n))
+`;
+
+val cl_kcomp_exentry_lem = store_thm("cl_kcomp_exentry_lem", ``
+!s s' n. cl_kcomp s s' n ==> cl_exentry s
+``,
+  Induct_on `n` 
+  >| [(* n = 0 *)
+      ONCE_REWRITE_TAC [cl_kcomp_cases] >>
+      REPEAT STRIP_TAC >>
+      FULL_SIMP_TAC std_ss [numTheory.NOT_SUC]
+      ,
+      (* n -> SUC n *)
+      ONCE_REWRITE_TAC [cl_kcomp_cases] >>
+      REPEAT STRIP_TAC >>
+      FULL_SIMP_TAC std_ss [numTheory.INV_SUC] >>
+      RW_TAC std_ss [] >>
+      RES_TAC
+     ]
+);
+
+val cl_wrel_def = Define` cl_wrel s s' = 
+?n. cl_kcomp s s' n /\ (cl_mode s' = USER)`;
+
+val cl_wrel_exentry_lem = store_thm("cl_wrel_exentry_lem", ``
+!s s'. cl_wrel s s' ==> cl_exentry s
+``,
+  RW_TAC std_ss [cl_wrel_def] >>
+  IMP_RES_TAC cl_kcomp_exentry_lem
+);
+
+val cl_wrel_mode_lem = store_thm("cl_wrel_mode_lem", ``
+!s s'. cl_wrel s s' ==> (cl_mode s = PRIV) /\ (cl_mode s' = USER)
+``,
+  RW_TAC std_ss [cl_wrel_def]
+  >| [(* PRIV *)
+      IMP_RES_TAC cl_kcomp_exentry_lem >>
+      FULL_SIMP_TAC std_ss [cl_exentry_def, cl_mode_def, 
+			    coreIfTheory.exentry_spec]
+      ,
+      (* USER *)
+      ASM_REWRITE_TAC []
+     ]      
+);
+
+
+
+(*********** finish ************)
+
+val _ = export_theory();
